add non-function closure summary helpers

rocq/theories/TypeSystem/EnvRuntimeBaseSafety.v
@@ -74,6 +74,104 @@ Proof.
     + apply IH. exact Hlookup.
 Qed.
 
+Fixpoint non_function_value_ty_b (T : Ty) : bool :=
+  match T with
+  | MkTy _ (TFn _ _) => false
+  | MkTy _ (TClosure _ _ _) => false
+  | MkTy _ (TForall _ _ body) => non_function_value_ty_b body
+  | MkTy _ (TTypeForall _ _ body) => non_function_value_ty_b body
+  | _ => true
+  end.
+
+Lemma non_function_value_ty_b_fn_value_ty :
+  forall f,
+    non_function_value_ty_b (fn_value_ty f) = false.
+Proof.
+  intros f.
+  unfold non_function_value_ty_b, fn_value_ty, fn_signature_ty_with_usage.
+  destruct (fn_type_params f); destruct (fn_lifetimes f); simpl; reflexivity.
+Qed.
+
+Lemma ty_compatible_non_function_value_ty_b :
+  forall Ω T_actual T_expected,
+    ty_compatible Ω T_actual T_expected ->
+    non_function_value_ty_b T_expected = true ->
+    non_function_value_ty_b T_actual = true.
+Proof.
+  intros Ω T_actual T_expected Hcompat.
+  induction Hcompat; simpl; intros Hnonfn; try discriminate; auto.
+  - subst. exact Hnonfn.
+Qed.
+
+Lemma ty_lifetime_equiv_non_function_value_ty_b :
+  forall T_actual T_expected,
+    ty_lifetime_equiv T_actual T_expected ->
+    non_function_value_ty_b T_expected = true ->
+    non_function_value_ty_b T_actual = true.
+Proof.
+  intros T_actual T_expected Hequiv.
+  induction Hequiv; simpl; intros Hnonfn; try discriminate; auto.
+Qed.
+
+Lemma value_has_type_empty_closure_non_function_value_ty_b_false :
+  forall env s fname T,
+    value_has_type env s (VClosure fname []) T ->
+    non_function_value_ty_b T = false.
+Proof.
+  intros env s fname T Htyped.
+  remember (VClosure fname []) as v eqn:Hv.
+  induction Htyped; try discriminate.
+  - apply non_function_value_ty_b_fn_value_ty.
+  - apply non_function_value_ty_b_fn_value_ty.
+  - assert (Hactual : non_function_value_ty_b T_actual = false) by auto.
+    destruct (non_function_value_ty_b T_expected) eqn:Hexpected; auto.
+    pose proof (ty_compatible_non_function_value_ty_b
+      Ω T_actual T_expected H Hexpected) as Hactual_true.
+    rewrite Hactual in Hactual_true. discriminate.
+  - assert (Hactual : non_function_value_ty_b T_actual = false) by auto.
+    destruct (non_function_value_ty_b T_expected) eqn:Hexpected; auto.
+    pose proof (ty_lifetime_equiv_non_function_value_ty_b
+      T_actual T_expected H Hexpected) as Hactual_true.
+    rewrite Hactual in Hactual_true. discriminate.
+Qed.
+
+Lemma value_has_type_non_function_value_summary :
+  forall env s v T,
+    value_has_type env s v T ->
+    non_function_value_ty_b T = true ->
+    value_function_closure_targets_summary env v.
+Proof.
+  intros env s v T Htyped Hnonfn.
+  destruct v; simpl; auto.
+  destruct l as [| se captured]; simpl; auto.
+  pose proof (value_has_type_empty_closure_non_function_value_ty_b_false
+    env s i T Htyped) as Hfalse.
+  rewrite Hnonfn in Hfalse. discriminate.
+Qed.
+
+Lemma store_function_closure_targets_summary_add_value_summary :
+  forall env s x T v,
+    store_function_closure_targets_summary env s ->
+    value_function_closure_targets_summary env v ->
+    store_function_closure_targets_summary env (store_add x T v s).
+Proof.
+  unfold store_function_closure_targets_summary, store_add.
+  intros env s x T v Hsummary Hvalue.
+  constructor; auto.
+Qed.
+
+Lemma store_function_closure_targets_summary_add_non_function :
+  forall env s x T v,
+    store_function_closure_targets_summary env s ->
+    value_has_type env s v T ->
+    non_function_value_ty_b T = true ->
+    store_function_closure_targets_summary env (store_add x T v s).
+Proof.
+  intros env s x T v Hsummary Htyped Hnonfn.
+  apply store_function_closure_targets_summary_add_value_summary; auto.
+  eapply value_has_type_non_function_value_summary; eassumption.
+Qed.
+
 Lemma initial_root_env_for_params_covers :
   forall ps,
     root_env_covers_params ps (initial_root_env_for_params ps).
